DynamoDbEncryption/runtimes/java/src/main/smithy-generated/software/amazon/cryptography/dbencryptionsdk/structuredencryption/model/ResolveAuthActionsOutput.java
@@ -1,0 +1,65 @@
+// Copyright Amazon.com Inc. or its affiliates. All Rights Reserved.
+// SPDX-License-Identifier: Apache-2.0
+// Do not modify this file. This file is machine generated, and any changes to it will be overwritten.
+package software.amazon.cryptography.dbencryptionsdk.structuredencryption.model;
+
+import java.util.List;
+import java.util.Objects;
+
+public class ResolveAuthActionsOutput {
+
+  private final List<CryptoItem> cryptoActions;
+
+  protected ResolveAuthActionsOutput(BuilderImpl builder) {
+    this.cryptoActions = builder.cryptoActions();
+  }
+
+  public List<CryptoItem> cryptoActions() {
+    return this.cryptoActions;
+  }
+
+  public Builder toBuilder() {
+    return new BuilderImpl(this);
+  }
+
+  public static Builder builder() {
+    return new BuilderImpl();
+  }
+
+  public interface Builder {
+    Builder cryptoActions(List<CryptoItem> cryptoActions);
+
+    List<CryptoItem> cryptoActions();
+
+    ResolveAuthActionsOutput build();
+  }
+
+  static class BuilderImpl implements Builder {
+
+    protected List<CryptoItem> cryptoActions;
+
+    protected BuilderImpl() {}
+
+    protected BuilderImpl(ResolveAuthActionsOutput model) {
+      this.cryptoActions = model.cryptoActions();
+    }
+
+    public Builder cryptoActions(List<CryptoItem> cryptoActions) {
+      this.cryptoActions = cryptoActions;
+      return this;
+    }
+
+    public List<CryptoItem> cryptoActions() {
+      return this.cryptoActions;
+    }
+
+    public ResolveAuthActionsOutput build() {
+      if (Objects.isNull(this.cryptoActions())) {
+        throw new IllegalArgumentException(
+          "Missing value for required field `cryptoActions`"
+        );
+      }
+      return new ResolveAuthActionsOutput(this);
+    }
+  }
+}
